okasaki/RedBlackSet_proof.v
@@ -24,12 +24,6 @@ Definition node_color e :=
   | Node col _ _ _ => col
   end.
 
-Definition case_color col (A:Type) (vred vblack:A) :=
-  match col with
-  | Red => vred
-  | Black => vblack
-  end.  
-
 Definition is_lt (X Y:T) := Y < X.
 Definition is_gt (X Y:T) := X < Y.
 
@@ -40,8 +34,11 @@ Inductive inv : bool -> nat -> set -> LibSet.set T -> Prop :=
       inv true m a A -> inv true m b B -> rep y Y ->
       foreach (is_lt Y) A -> foreach (is_gt Y) B ->
       E = (\{Y} \u A \u B) ->
-      (rr -> col = Black \/ (node_color a = Black /\ node_color b = Black)) ->
-      (n =' case_color col m (S m)) ->
+      (if rr then match col with 
+         | Black => True 
+         | Red => node_color a = Black /\ node_color b = Black
+         end else True) ->
+      (n =' match col with Black => S m | Red => m end) ->
       inv rr n (Node col a y b) E.
 
 (** model *)
@@ -57,11 +54,9 @@ Defined.
 (** automation *)
 
 Hint Constructors inv.
-
 Hint Extern 1 (_ = _ :> LibSet.set _) => permut_simpl : set.
 
 Definition U := LibSet.set T.
-
 Ltac myauto cont :=
   match goal with 
   | |- _ = _ :> LibSet.set ?T => try solve [ change (LibSet.set T) with U; cont tt ]
@@ -72,6 +67,9 @@ Ltac auto_tilde ::= myauto ltac:(fun _ => eauto).
 Ltac auto_star ::= try solve [ intuition (eauto with set) ].
 Hint Extern 1 (@lt nat _ _ _) => simpl; math.
 
+Ltac my_intuit := 
+  rew_foreach in *; intuit; tryfalse.
+
 (** useful facts *)
 
 Fixpoint size t :=
@@ -80,13 +78,29 @@ Fixpoint size t :=
   | Node _ a _ b => (1 + size a + size b)%nat
   end.
 
-Lemma inv_weaken : forall n E e,
-  inv true n e E -> inv false n e E.
+Definition case_color col (A:Type) (vred vblack:A) :=
+  match col with
+  | Red => vred
+  | Black => vblack
+  end.  
+
+Lemma inv_weaken : forall b n E e,
+  inv b n e E -> inv false n e E.
 Proof. introv RepE. inverts* RepE. Qed.
+
+Lemma inv_weaken' : forall (b' b : bool) n E e,
+  inv b n e E -> (b' -> b) -> inv b' n e E.
+Proof.
+  introv RepE N. destruct b; destruct b'; auto.
+  inverts* RepE. false~ N.
+Qed.
 
 Lemma inv_strengthen : forall n E col a x b,
   inv false n (Node col a x b) E ->
-  (col = Black \/ (node_color a = Black /\ node_color b = Black)) ->
+  match col with 
+  | Black => True 
+  | Red => node_color a = Black /\ node_color b = Black
+  end ->
   inv true n (Node col a x b) E.
 Proof. introv RepE H. inverts* RepE. Qed.
 
@@ -112,11 +126,6 @@ Proof. intros. apply~ foreach_weaken. intros_all. apply* my_lt_trans. Qed.
 
 Hint Resolve foreach_lt_trans foreach_gt_trans.
 
-(** local tactics *)
-
-Ltac my_intuit := 
-  intuit; try rewrite foreach_single_eq in *.
-
 (** verification *)
 
 Lemma empty_spec : rep empty \{}.
@@ -137,10 +146,10 @@ Proof.
   iff M. auto. set_in M.
     subst. false~ (lt_irrefl Y).
     auto.
-    false. applys* (@foreach_gt_notin B).
+    false* (@foreach_gt_notin B).
   iff M. auto. set_in M. 
     subst. false~ (lt_irrefl Y). 
-    false. applys* (@foreach_lt_notin A).
+    false* (@foreach_lt_notin A).
     auto.
   asserts_rewrite~ (X = Y). apply~ nlt_nslt_to_eq. 
 Qed.
@@ -153,82 +162,70 @@ Lemma balance_spec :
   forall i1 i2 n E1 E2 X,
   rep x X -> inv i1 n e1 E1 -> inv i2 n e2 E2 -> 
   foreach (is_lt X) E1 -> foreach (is_gt X) E2 ->
-  case_color col (i1 /\ i2) (Xor i1 i2) ->
-  R (fun e => inv (case_color col false true) (case_color col n (S n)) e (\{X} \u E1 \u E2)).
+  match col with Black => xor i1 i2 | Red => i1 /\ i2 end ->
+  R (fun e => inv (match col with Black => true | Red => false end)
+                  (match col with Black => S n | Red => n end)
+                  e (\{X} \u E1 \u E2)).
 Proof. 
-  xcf. intros [[[c e1] x] e2]. xisspec. (* todo improve *)
-  intros [[[col e1] x] e2]. introv RepX Inv1 Inv2 GtX LtX Ixor.
-   xgo; simpl in Ixor.
+  xcf; intros [[[c e1] x] e2]. xisspec.
+  introv RepX I1 I2 GtX LtX Ixor. xgo.
   (* balance 1 *)
-  xcleanpat. inverts Inv1. inverts H3. simpls. subst.
-  destruct Ixor as [[? ?]|[? ?]]; substb i1 i2.
-  destruct H12 as [|[? ?]]; auto_false.
-  rew_foreach H6. rew_foreach GtX. my_intuit.
+  xcleanpat. inverts I1 as IA IB. inverts IA. subst.
+  destruct (xor_cases Ixor) as [M|M]; destruct M; subst i1 i2; my_intuit.
   applys* (>>> inv_node (\{Y0} \u A0 \u B0) Y (\{X} \u B \u E2)). 
   (* balance 2 *) 
-  xcleanpat. inverts Inv1. inverts H4. simpls. subst.
-  destruct Ixor as [[? ?]|[? ?]]; substb i1 i2.
-  destruct H12 as [|[? ?]]; auto_false.
-  rew_foreach H9. rew_foreach GtX. my_intuit.
+  xcleanpat. inverts I1 as IA IB. inverts IB. subst.
+  destruct (xor_cases Ixor) as [M|M]; destruct M; subst i1 i2; my_intuit.
   applys* (>>> inv_node (\{Y} \u A \u A0) Y0 (\{X} \u B0 \u E2)). 
   (* balance 3 *) 
-  xcleanpat. inverts Inv2. inverts H3. simpls. subst.
-  destruct Ixor as [[? ?]|[? ?]]; substb i1 i2.
-  rew_foreach H6. rew_foreach LtX. my_intuit.
+  xcleanpat. inverts I2 as IA IB. inverts IA. subst.
+  destruct (xor_cases Ixor) as [M|M]; destruct M; subst i1 i2; my_intuit.
   applys* (>>> inv_node (\{X} \u E1 \u A0) Y0 (\{Y} \u B0 \u B)). 
-  destruct H12 as [|[? ?]]; auto_false.
   (* balance 4 *) 
-  xcleanpat. inverts Inv2. inverts H4. simpls. subst.
-  destruct Ixor as [[? ?]|[? ?]]; substb i1 i2.
-  rew_foreach H10. rew_foreach LtX. my_intuit.
+  xcleanpat. inverts I2 as IA IB. inverts IB. subst.
+  destruct (xor_cases Ixor) as [M|M]; destruct M; subst i1 i2; my_intuit.
   applys* (>>> inv_node (\{X} \u E1 \u A) Y (\{Y0} \u A0 \u B0)). 
-  destruct H12 as [|[? ?]]; auto_false.
   (* no balance *)
-  destruct col; simpls.
-    destruct Ixor. rewrite H in Inv1. rewrite H0 in Inv2. econstructor; auto_false*. 
-    cuts Inv1' Inv2': (inv true n e1 E1 /\ inv true n e2 E2). econstructor; eauto.
-    destruct Ixor as [[? ?]|[? ?]]; substb i1 i2; split.
-      auto.
-      inversions keep Inv2. auto~. apply~ inv_strengthen.
-        destruct~ col. right. split. 
+  destruct c.
+    destruct Ixor. substb i1. substb i2. constructors~.
+    destruct (xor_cases Ixor) as [M|M]; destruct M; subst i1 i2.
+      inverts keep I2; auto~. constructors~. apply~ inv_strengthen.
+        destruct~ col. split. 
           destruct~ a. destruct~ c. false~ C1.
           destruct~ b. destruct~ c. false~ C2.
-      inversions keep Inv1. auto~. apply~ inv_strengthen.
-        destruct~ col. right. split.
+      inverts keep I1; auto~. constructors~. apply~ inv_strengthen.
+        destruct~ col. split. 
           destruct~ a. destruct~ c. false~ C.
           destruct~ b. destruct~ c. false~ C0.
-      auto. 
 Qed.
 
 Hint Extern 1 (RegisterSpec balance) => Provide balance_spec.
+
+Definition ins_spec X ins :=
+  Spec ins e |R>>
+    forall n E, inv true n e E -> 
+    R (fun e' => inv (match node_color e with Black => true | Red => false end)
+                     n e' (\{X} \u E)).
 
 Lemma insert_spec : RepTotal insert (X;elem) (E;set) >>
   \{X} \u E ; set.
 Proof. 
   xcf. introv RepX (n&InvE&HeB).
-  xfun_induction_nointro (fun ins => Spec ins e |R>>
-    forall n E, inv true n e E -> 
-    R (fun e' => inv (case_color (node_color e) false true) n e' (\{X} \u E)))
-   size.
-    clears s n E. intros e IH n E InvE. inverts InvE as.
-    xgo*.
-    introv InvA InvB RepY GtY LtY Cinv Ninv.
+  xfun_induction_nointro (ins_spec X) size.
+    clears s n E. intros e IH n E InvE. inverts InvE as. xgo*.
+    simple*.
+    introv InvA InvB RepY GtY LtY Col Num.
     xgo~ '_x4 XstopAfter, '_x3 XstopAfter.
-    destruct (node_color a); simpls.
-      xgo~. destruct~ Cinv as [Imp|[Ha Hb]]; auto_false. subst col. simple*.
-        intros e InvE. equates* 1 3.
-      xapp~ (case_color col true false) (\{X} \u A) B.
-        destruct col; simpl. eauto. apply* inv_weaken.
-        destruct col; simple*.
-        intros e InvE. equates* 1 3. 
-    destruct (node_color b); simpls.
-      xapp~. destruct~ Cinv as [Imp|[Ha Hb]]; auto_false. subst col. simple*.
-        intros e InvE. equates* 1 3.
-      xapp~ true (case_color col true false) A (\{X} \u B).
-        destruct col; simpl. eauto. apply* inv_weaken.
-        destruct col; simple*.
-        intros e InvE. equates* 1 3.
-    asserts_rewrite~ (X = Y). apply~ nlt_nslt_to_eq. subst s. auto*.
+    forwards~ M: (>>> inv_weaken' (match col with Black => false | Red => true end)).
+      intro; destruct col; destruct (node_color a); destruct Col; tryfalse; auto.
+     clear P_x4. xapp~. destruct~ col.
+     ximpl as e. simpl. destruct col; subst; equates* 1.
+    forwards~ M: (>>> inv_weaken' (match col with Black => false | Red => true end)).
+      intro; destruct col; destruct (node_color b); destruct Col; tryfalse; auto.
+     clear P_x3. xapp~. destruct~ col.
+     ximpl as e. simpl. destruct col; subst; equates* 1.
+    asserts_rewrite~ (X = Y). apply~ nlt_nslt_to_eq.
+      subst s. simpl. destruct col; constructors*.
   xlet. xapp~. inverts P_x5; xgo.
     fset_inv.
     exists* __.
